work on pl stuff

src/indexing.v
@@ -15,37 +15,121 @@ Definition plend (pl: PathLoc) := match pl with (_, l) => l end.
 
 Section Indexing.
 
-(*Context {M: Type}  `{!EqDecision M, !Countable M}.*)
+(*Context {M: Type}  `{!EqDecision M}.*)
 (*Context `{!EqDecision RefinementIndex}.
 Context {refinement_of_index : RefinementIndex -> Refinement M M}.*)
 
-Definition node_of_pl {M} `{!EqDecision M, !Countable M, !TPCM M}
-    (branch: Branch M) (pl: PathLoc) : Node M. Admitted.
+Context {M} `{!EqDecision M, !TPCM M}.
+
+Fixpoint branch_step_branch (branch: Branch M) (idx: nat) :=
+  match branch, idx with
+  | BranchNil, _ => BranchNil
+  | BranchCons _ sub, (S idx) => branch_step_branch sub idx
+  | BranchCons (CellNode _ b) _, 0 => b
+  end.
+  
+Definition triv_cell : Cell M := CellCon unit empty.
+Definition triv_node : Node M := CellNode triv_cell BranchNil.
+
+Fixpoint branch_step_node (branch: Branch M) (idx: nat) :=
+  match branch, idx with
+  | BranchNil, _ => triv_node
+  | BranchCons _ sub, (S idx) => branch_step_node sub idx
+  | BranchCons n _, 0 => n
+  end.
+  
+Fixpoint node_of_pl' (branch: Branch M) (p: list nat) (i: nat) : Node M :=
+  match p with
+  | [] => branch_step_node branch i
+  | (x :: p0) => node_of_pl' (branch_step_branch branch x) p0 i
+  end.
+  
+Definition node_of_pl (branch: Branch M) (pl: PathLoc) : Node M :=
+  match pl with
+  | (p, i) => node_of_pl' branch p i
+  end.
     
-Definition cell_of_pl {M} `{!EqDecision M, !Countable M, !TPCM M}
-    (branch: Branch M) (pl: PathLoc) : Cell M := match node_of_pl branch pl with CellNode c _ => c end.
+Definition cell_of_pl (branch: Branch M) (pl: PathLoc) : Cell M :=
+  match node_of_pl branch pl with CellNode c _ => c end.
     
-Definition every_node {M} `{!EqDecision M, !Countable M, !TPCM M}
+    (*
+Definition every_node {M} `{!EqDecision M, !TPCM M}
     (branch: Branch M) (fn : Node M -> nat -> Prop) : Prop. Admitted.
 
-Lemma every_node_equiv_forall {M} `{!EqDecision M, !Countable M, !TPCM M}
+Lemma every_node_equiv_forall {M} `{!EqDecision M, !TPCM M}
     (branch : Branch M) (fn : Node M -> nat -> Prop)
     (rtriv: ∀ n idx , node_trivial n -> fn n idx)
   : (every_node branch fn) <-> (forall pl , fn (node_of_pl branch pl) (plend pl)). Admitted.
+  *)
+  
+Lemma node_trivial_triv_node : node_trivial triv_node.
+Proof. unfold node_trivial, triv_node, cell_trivial, triv_cell. crush.
+Qed.
+  
+Lemma branch_step_node_op branch1 branch2 i
+  : branch_step_node branch1 i ⋅ branch_step_node branch2 i
+      ≡ branch_step_node (branch1 ⋅ branch2) i.
+Proof.
+  generalize branch1, branch2. clear branch1. clear branch2.
+  induction i.
+  - intros. unfold "⋅", node_op, branch_op, branch_step_node. destruct branch1, branch2.
+     + unfold "⋅". trivial.
+     + apply op_trivial_node. apply node_trivial_triv_node.
+     + setoid_rewrite node_op_comm.
+       apply op_trivial_node. apply node_trivial_triv_node.
+     + apply op_trivial_node. apply node_trivial_triv_node.
+  - intros. unfold "⋅", node_op, branch_op, branch_step_node. destruct branch1, branch2.
+     + fold branch_step_node. fold node_op. apply IHi.
+     + fold branch_step_node. fold node_op.
+        setoid_rewrite op_trivial_node; trivial. apply node_trivial_triv_node.
+     + fold branch_step_node. fold node_op.
+        setoid_rewrite node_op_comm.
+        setoid_rewrite op_trivial_node; trivial. apply node_trivial_triv_node.
+     + fold branch_step_node. fold node_op.
+        setoid_rewrite op_trivial_node; trivial. apply node_trivial_triv_node.
+Qed.
 
-Lemma forall_node_op {M} `{!EqDecision M, !Countable M, !TPCM M}
-    (branch1 : Branch M) (branch2 : Branch M)
-  : forall pl , (node_of_pl branch1 pl) ⋅ (node_of_pl branch2 pl) ≡ node_of_pl (branch1 ⋅ branch2) pl.
-Admitted.
+Lemma branch_step_branch_op branch1 branch2 i
+  : branch_step_branch branch1 i ⋅ branch_step_branch branch2 i
+      ≡ branch_step_branch (branch1 ⋅ branch2) i.
+Proof.
+  generalize branch1, branch2. clear branch1. clear branch2.
+  induction i.
+  - intros. unfold "⋅". unfold branch_op, branch_step_node. destruct branch1, branch2.
+     + fold branch_op. unfold branch_step_branch. destruct n. destruct n0. unfold "⋅".
+        trivial.
+     + fold branch_op. cbn [branch_step_branch]. destruct n. apply op_trivial_branch.
+        unfold branch_trivial. trivial.
+     + fold branch_op. cbn [branch_step_branch]. destruct n. unfold branch_op. trivial.
+     + fold branch_op. cbn [branch_step_branch]. unfold branch_op. trivial.
+  - intros. unfold "⋅". unfold node_op, branch_op, branch_step_branch. destruct branch1, branch2.
+     + destruct n. destruct n0. fold branch_op. fold branch_step_branch. fold node_op. unfold "⋅". unfold node_op. apply IHi.
+     + destruct n. fold branch_op. fold branch_step_branch.
+        setoid_rewrite op_trivial_branch; trivial. unfold branch_trivial. trivial.
+     + destruct n. fold branch_op. fold branch_step_branch. trivial.
+     + trivial.
+Qed.
 
-Lemma forall_cell_op {M} `{!EqDecision M, !Countable M, !TPCM M}
+Lemma node_of_pl_op (branch1 : Branch M) (branch2 : Branch M) pl
+  : (node_of_pl branch1 pl) ⋅ (node_of_pl branch2 pl) ≡ node_of_pl (branch1 ⋅ branch2) pl.
+Proof.
+  generalize branch1, branch2. clear branch1. clear branch2.
+  destruct pl. rename l into p. rename n into i.
+  induction p.
+  - intros. unfold node_of_pl, node_of_pl'. apply branch_step_node_op.
+  - intros.
+      unfold node_of_pl in *. cbn [node_of_pl'].
+      setoid_rewrite <- branch_step_branch_op.
+  
+
+Lemma cell_of_pl_op {M} `{!EqDecision M, !TPCM M}
     (branch1 : Branch M) (branch2 : Branch M)
   : forall pl , (cell_of_pl branch1 pl) ⋅ (cell_of_pl branch2 pl) ≡ cell_of_pl (branch1 ⋅ branch2) pl.
 Admitted.
 
 
 
-Lemma equiv_extensionality_cells {M} `{!EqDecision M, !Countable M, !TPCM M}
+Lemma equiv_extensionality_cells {M} `{!EqDecision M, !TPCM M}
     (branch1: Branch M) (branch2: Branch M)
     (ext_eq : forall pl , (cell_of_pl branch1 pl) ≡ (cell_of_pl branch2 pl))
     : branch1 ≡ branch2. Admitted.
